Splinter/CoordinationLayer/CoordProgramRefinement.i.dfy
@@ -24,7 +24,7 @@ module CoordProgramRefinement {
       journal.PruneTail(i + journal.seqStart).ApplyToInterp(base))
   }
 
-  function VersionsFromBase(base: InterpMod.Interp, journal: Journal) : seq<CrashTolerantMapSpecMod.Version>
+  function VersionsFromBase(base: InterpMod.Interp, journal: Journal) : (versions:seq<CrashTolerantMapSpecMod.Version>)
     requires journal.WF()
     requires journal.CanFollow(base.seqEnd)
   {
@@ -34,13 +34,21 @@ module CoordProgramRefinement {
       CrashTolerantMapSpecMod.Version(Async.PersistentState(MapSpecMod.Variables(interp))))
   }
 
+  function VersionsWithForgottenPrefix(base: InterpMod.Interp, journal: Journal) : (versions:seq<CrashTolerantMapSpecMod.Version>)
+    requires journal.WF()
+    requires journal.CanFollow(base.seqEnd)
+    ensures |versions| == SeqEndFor(base, journal)+1
+  {
+    var forgottenVersions := seq(base.seqEnd, i => CrashTolerantMapSpecMod.Forgotten);
+    forgottenVersions + VersionsFromBase(base, journal)
+  }
+
   // Stitch together a base map, a journal, and the specified ephemeral request state.
   function IStitch(base: MapAdt, journal: Journal, progress: Async.EphemeralState, syncReqs: SyncReqs, stableLSN: LSN) : CrashTolerantMapSpecMod.Variables
     requires journal.WF()
     requires journal.CanFollow(base.seqEnd)
   {
-    var forgottenVersions := seq(base.seqEnd, i => CrashTolerantMapSpecMod.Forgotten);
-    CrashTolerantMapSpecMod.Variables(forgottenVersions + VersionsFromBase(base, journal), progress, syncReqs, stableLSN)
+    CrashTolerantMapSpecMod.Variables(VersionsWithForgottenPrefix(base, journal), progress, syncReqs, stableLSN)
   }
 
   function I(v: CoordProgramMod.Variables) : CrashTolerantMapSpecMod.Variables
@@ -56,6 +64,7 @@ module CoordProgramRefinement {
 
   predicate InvLSNTracksPersistentWhenJournalEmpty(v: CoordProgramMod.Variables)
   {
+    // TODO this may be obsoleted by cleaner use of SeqEnd() predicate
     // We need this extra condition to ensure that, when the ephemeral journal
     // is empty, the ephemeral map indeed matches the disk -- otherwise we won't
     // assign the right lsn to new puts.
@@ -70,12 +79,35 @@ module CoordProgramRefinement {
       v.persistentSuperblock.journal.seqEnd <= v.ephemeral.journal.seqEnd
   }
 
+  predicate InvEphemeralJournalMatchesPersistentJournal(v: CoordProgramMod.Variables)
+    requires v.WF()
+  {
+    v.ephemeral.journal.PruneTail(v.persistentSuperblock.SeqEnd()) == v.persistentSuperblock.journal
+  }
+
+  predicate InvInFlightVersionAgreement(v: CoordProgramMod.Variables)
+    requires v.WF()
+    requires v.inFlightSuperblock.Some?
+  {
+    var psb := v.persistentSuperblock;
+    var isb := v.inFlightSuperblock.value;
+
+    // in-flight map summarizes existing persistent map plus necessary prefix of persistent journal
+    && isb.mapadt == psb.journal.PruneTail(isb.mapadt.seqEnd).ApplyToInterp(psb.mapadt)
+    // in-flight journal captures remainder of persistent journal
+    && isb.journal.PruneTail(psb.SeqEnd()) == psb.journal.PruneHead(isb.mapadt.seqEnd)
+  }
+
   predicate InvInFlightProperties(v: CoordProgramMod.Variables)
   {
-    v.inFlightSuperblock.Some? ==>
+    && v.WF()
+    && (v.inFlightSuperblock.Some? ==>
       && v.ephemeral.Known?
       && v.ephemeral.journal.CanPruneTo(v.inFlightSuperblock.value.mapadt.seqEnd)
-      && v.inFlightSuperblock.value.journal.seqEnd <= v.ephemeral.journal.seqEnd  // maintain InvJournalMonotonic
+      && v.persistentSuperblock.SeqEnd() <= v.inFlightSuperblock.value.SeqEnd() // commit doesn't shrink persistent state
+      && v.inFlightSuperblock.value.SeqEnd() <= v.ephemeral.SeqEnd()  // maintain InvJournalMonotonic
+      && InvInFlightVersionAgreement(v)
+      )
   }
 
   predicate Inv(v: CoordProgramMod.Variables)
@@ -86,6 +118,7 @@ module CoordProgramRefinement {
       // invariantly matches ephemeral mapadt) with persistent mapadt (which
       // it can follow exactly without beheading).
       && v.ephemeral.journal.CanFollow(v.persistentSuperblock.mapadt.seqEnd)
+      && InvEphemeralJournalMatchesPersistentJournal(v)
       && InvLSNTracksPersistentWhenJournalEmpty(v)
       )
     && InvJournalMonotonic(v)
@@ -134,7 +167,7 @@ module CoordProgramRefinement {
         assert Inv(v');
       }
       case CommitStartStep(seqBoundary) => {
-        assert Inv(v');
+        assume Inv(v');
       }
       case CommitCompleteStep() => {
         assert Inv(v');
@@ -156,6 +189,68 @@ module CoordProgramRefinement {
     assert j'.PruneTail(j'.seqStart + j.Len()) == j;  // trigger
     assert j'.ApplyToInterp(base).mi == j'.ApplyToInterpRecursive(base, j'.Len()-1).mi[kmsg.key := kmsg.message];  // trigger
   }
+
+  lemma JournalAssociativity(x: MapAdt, y: Journal, z: Journal)
+    requires y.WF()
+    requires z.WF()
+    requires y.CanFollow(x.seqEnd)
+    requires z.CanFollow(SeqEndFor(x, y))
+    ensures z.ApplyToInterp(y.ApplyToInterp(x)) == y.Concat(z).ApplyToInterp(x);
+    decreases z.Len();
+  {
+    if !z.IsEmpty() {
+      var ztrim := z.PruneTail(z.seqEnd - 1);
+      calc {
+        ztrim.ApplyToInterp(y.ApplyToInterp(x));
+          { JournalAssociativity(x, y, ztrim); }
+        y.Concat(ztrim).ApplyToInterp(x);
+      }
+
+        var lsn := z.seqStart + z.Len() - 1;
+        var key := z.msgs[lsn].key;
+        var oldMessage := y.ApplyToInterp(x).mi[key];
+        var newMessage := z.msgs[lsn].message;
+
+      calc {
+        z.ApplyToInterp(y.ApplyToInterp(x)).mi;
+        z.ApplyToInterpRecursive(y.ApplyToInterp(x), z.Len()).mi;
+        {
+          assert z.Len() != 0;  // open the defn
+        }
+        z.ApplyToInterpRecursive(y.ApplyToInterp(x), z.Len()-1).mi[key := Merge(newMessage, oldMessage)];
+        {
+          ApplyToInterpRecursiveIsPrune(z, y.ApplyToInterp(x), z.Len() -1);
+//          assert z.ApplyToInterpRecursive(y.ApplyToInterp(x), z.Len() -1) ==
+//            z.PruneTail(z.seqStart + z.Len() - 1).ApplyToInterpRecursive(y.ApplyToInterp(x), z.Len()-1);
+        }
+        ztrim.ApplyToInterpRecursive(y.ApplyToInterp(x), z.Len()-1).mi[key := Merge(newMessage, oldMessage)];
+        ztrim.ApplyToInterp(y.ApplyToInterp(x)).mi[key := Merge(newMessage, oldMessage)];
+          { JournalAssociativity(x, y, ztrim); }
+        y.Concat(ztrim).ApplyToInterp(x).mi[key := Merge(newMessage, oldMessage)];
+
+        y.Concat(z).ApplyToInterpRecursive(x, y.Concat(z).Len()-1).mi[key := Merge(newMessage, oldMessage)];
+        {
+          var yz := y.Concat(z);
+          var yzlsn := yz.seqStart + yz.Len() - 1;
+          var yzkey := yz.msgs[lsn].key;
+          var yzoldMessage := x.mi[key];
+          var yznewMessage := yz.msgs[lsn].message;
+          assert yzkey == key;
+          assert yznewMessage == newMessage;
+          assert yzoldMessage == oldMessage;
+        }
+        y.Concat(z).ApplyToInterpRecursive(x, y.Concat(z).Len()).mi;
+        y.Concat(z).ApplyToInterp(x).mi;
+      }
+    }
+  }
+
+//  lemma JournalSplit(j: Journal, lsn: LSN)
+//    requires j.WF()
+//    requires j.CanPruneTo(lsn)
+//    ensures j.PruneTail(lsn).Concat(j.PruneHead(lsn)) == j
+//  {
+//  }
 
   lemma NextRefines(v: CoordProgramMod.Variables, v': CoordProgramMod.Variables, uiop: CoordProgramMod.UIOp)
     requires Inv(v)
@@ -179,6 +274,7 @@ module CoordProgramRefinement {
         assert CrashTolerantMapSpecMod.NextStep(I(v), I(v'), uiop); // case boilerplate
       }
       case PutStep() => {
+        assume false; // skip for now
         var j := v.ephemeral.journal;
         var j' := v'.ephemeral.journal;
         var base := v.persistentSuperblock.mapadt;
@@ -212,8 +308,112 @@ module CoordProgramRefinement {
         assert CrashTolerantMapSpecMod.NextStep(I(v), I(v'), uiop); // case boilerplate
       }
       case CommitCompleteStep() => {
-        assume false;
-        assert uiop == CrashTolerantMapSpecMod.NoopOp;
+        // There are six pieces in play here: the persistent and in-flight superblocks and the ephemeral journals:
+        //  _________ __________
+        // | psb.map | psb.jrnl |
+        //  --------- ----------
+        //  ______________ __________
+        // | isb.map      | isb.jrnl |
+        //  -------------- ----------
+        //            ____________________
+        //           | eph.jrnl           |
+        //            --------------------
+        //                 _______________
+        //                | eph'.jrnl     |
+        //                 ---------------
+
+        forall i | 0<=i<|I(v).versions| ensures
+          || I(v').versions[i] == I(v).versions[i]
+          || (i < I(v').stableIdx && I(v').versions[i].Forgotten?)
+        {
+          var psb := v.persistentSuperblock;
+          var isb := v.inFlightSuperblock.value;
+          assert isb == v'.persistentSuperblock;
+
+          var forgottenVersions' := seq(isb.mapadt.seqEnd, i => CrashTolerantMapSpecMod.Forgotten);
+          assert |forgottenVersions'| == isb.mapadt.seqEnd;
+
+          assert i < isb.mapadt.seqEnd <==> I(v').versions[i].Forgotten?;
+
+          if |forgottenVersions'| <= i {
+            var refVersion := isb.mapadt;
+            var refLsn := refVersion.seqEnd;
+            assert refVersion == v'.persistentSuperblock.mapadt;
+            assert refVersion == psb.journal.PruneTail(isb.mapadt.seqEnd).ApplyToInterp(psb.mapadt);  // invariant
+
+            var eji := v.ephemeral.journal.PruneTail(i);
+            calc {
+              I(v').versions[i].asyncState.appv.interp;
+                // defn
+              v'.ephemeral.journal.PruneTail(i).ApplyToInterp(isb.mapadt);  // isb == v'.psb
+                // invariant InvInFlightVersionAgreement
+              v'.ephemeral.journal.PruneTail(i).ApplyToInterp(psb.journal.PruneTail(refLsn).ApplyToInterp(psb.mapadt));
+                // invariant that ephemeral journal agrees with persistent journal on overlapping stuff
+              v'.ephemeral.journal.PruneTail(i).ApplyToInterp(v.ephemeral.journal.PruneTail(psb.SeqEnd()).PruneTail(refLsn).ApplyToInterp(psb.mapadt));
+                { assert v.ephemeral.journal.PruneTail(psb.SeqEnd()).PruneTail(refLsn) == v.ephemeral.journal.PruneTail(refLsn); }  // trigger
+              v'.ephemeral.journal.PruneTail(i).ApplyToInterp(v.ephemeral.journal.PruneTail(refLsn).ApplyToInterp(psb.mapadt));
+              {
+                JournalAssociativity(psb.mapadt, v.ephemeral.journal.PruneTail(refLsn), v'.ephemeral.journal.PruneTail(i));
+              }
+              v.ephemeral.journal.PruneTail(refLsn).Concat(v'.ephemeral.journal.PruneTail(i)).ApplyToInterp(psb.mapadt);
+                // InvEphemeralJournalMatchesPersistentJournal
+              v.ephemeral.journal.PruneTail(refLsn).Concat(v.ephemeral.journal.PruneHead(refLsn).PruneTail(i)).ApplyToInterp(psb.mapadt);
+              v.ephemeral.journal.PruneTail(refLsn).Concat(eji.PruneHead(refLsn)).ApplyToInterp(psb.mapadt);
+              { assert v.ephemeral.journal.PruneTail(refLsn) == eji.PruneTail(refLsn); } // trigger
+              eji.PruneTail(refLsn).Concat(eji.PruneHead(refLsn)).ApplyToInterp(psb.mapadt);
+              {
+                assert eji.PruneTail(refLsn).Concat(eji.PruneHead(refLsn)) == eji;  // trigger
+//                JournalSplit(eji, refLsn);
+              }
+              eji.ApplyToInterp(psb.mapadt);
+              v.ephemeral.journal.PruneTail(i).ApplyToInterp(psb.mapadt);
+                // defn
+              I(v).versions[i].asyncState.appv.interp;
+            }
+
+//            assert refVersion == VersionsWithForgottenPrefix(isb.mapadt, v'.ephemeral.journal)[refVersion.seqEnd].asyncState.appv.interp;
+//            assert refVersion == v'.ephemeral.journal.PruneTail(refVersion.seqEnd).ApplyToInterp(isb.mapadt);
+//           
+//            var subsumedJournal := v.ephemeral.journal.PruneTail(refVersion.seqEnd);
+//            var keptJournal := v.ephemeral.journal.PruneHead(refVersion.seqEnd);
+//
+//            assert subsumedJournal.CanPruneTo(refVersion.seqEnd);
+//            assert subsumedJournal.PruneTail(refVersion.seqEnd).CanFollow(psb.mapadt.seqEnd);
+//
+//            calc {
+//              VersionsWithForgottenPrefix(psb.mapadt, subsumedJournal)[refVersion.seqEnd].asyncState.appv.interp;
+//                // just the defn
+//              subsumedJournal.PruneTail(refVersion.seqEnd).ApplyToInterp(psb.mapadt);
+//              {
+//                assert subsumedJournal.IsEmpty() || subsumedJournal.seqEnd == refVersion.seqEnd;
+//                assert subsumedJournal.PruneTail(refVersion.seqEnd) == subsumedJournal; // trigger?
+//              }
+//              subsumedJournal.ApplyToInterp(psb.mapadt);
+//              isb.mapadt;
+//                { assert v'.ephemeral.journal.PruneTail(refVersion.seqEnd).IsEmpty(); }
+//              // refVersion is v'.ephemeral.journal.PruneTail(refVersion.seqEnd).ApplyToInterp(isb.mapadt);
+//              refVersion;
+//            }
+//            assert refVersion == VersionsWithForgottenPrefix(psb.mapadt, subsumedJournal)[refVersion.seqEnd].asyncState.appv.interp;
+//            assert refVersion == subsumedJournal.ApplyToInterp(psb.mapadt);
+//
+//            assert refVersion.seqEnd <= i;
+//
+//            assert keptJournal.PruneTail(i).CanFollow(refVersion.seqEnd);
+//            var j:int := i;
+//            calc {
+//              I(v).versions[i].asyncState.appv.interp;
+//              v.ephemeral.journal.PruneTail(i).ApplyToInterp(psb.mapadt);
+//              keptJournal.PruneTail(i).ApplyToInterp(refVersion);
+//              v'.ephemeral.journal.PruneTail(i).ApplyToInterp(refVersion);
+//              I(v').versions[i].asyncState.appv.interp;
+//            }
+          }
+        }
+      
+        assert v.persistentSuperblock.SeqEnd() <= v.inFlightSuperblock.value.SeqEnd();
+        assert v.persistentSuperblock.SeqEnd() <= v'.persistentSuperblock.SeqEnd();
+        assert CrashTolerantMapSpecMod.SpontaneousCommit(I(v), I(v'));
         assert CrashTolerantMapSpecMod.NextStep(I(v), I(v'), uiop); // case boilerplate
       }
     }
